Verse/Language.v
@@ -1,5 +1,5 @@
+Require Import Verse.Types.Internal.
 Require Import Verse.Types.
-Require Import Verse.TypeCons.
 Require Vector.
 Import List.ListNotations.
 Import String.
