Verse/Types/Internal.v
@@ -1,0 +1,123 @@
+Require Import String.
+Require Import Verse.Tactics.
+Require Import Verse.BinTree.
+Require Import Verse.Nibble.
+Require Import Verse.Error.
+
+(**
+
+* Types in verse.
+
+The assembly language supported by verse is typed. We have the
+words, vectors, array types and the type of sequences.
+
+** Values.
+
+Verse supports both scalar values and vector values. The scalar types
+that are supported are [Word8], [Word16], [Word32] and [Word64]. The
+type [Byte] is an aliase for [Word8]. The libary also supports 128 and
+256 vector types of each of the above type. For example,
+[Vector128_64] denotes a vector that consists of 2 64-bit word where
+as [Vector256_64] denotes the vector type that consists of 4 64-bit
+words. These are the standard vector and word types supported and
+users should use these in the code.
+
+Internally, the value [word n] denotes scalar values that are unsigned
+integers of [2^n] bytes. Vector of [2^m] elements, each of which are
+of type [word n] are captured by the type [vector m (word n)].
+However, users should stick to the standard vector and word types as
+much as possible.
+
+** Arrays.
+
+Arrays are abstractions to contiguous memory locations in the machine
+each of which can store a value. Arrays also required to specify the
+endianness of the values as it matters when loading or storing into
+memory.
+
+** Sequences.
+
+Cryptographic primitives like block cipher often process a stream of
+blocks. A sequence type abstracts such streams of block. The number of
+elements in a sequence is not know at compile time but its elements
+are required to be a bounded type, i.e. either a value or an array
+type.
+
+
+** The kind system.
+
+The type system has to rule out certain types like for example nested
+sequences or vector of arrays etc. A rudimentary kind system is
+implemented to avoid such errors. The kind system ensures the following
+restrictions.
+
+  - The type [vector t] is valid only for a scalar type [t], i.e. [t]
+    is a word type.
+
+  - The array of type [t] is valid if and only if the type [t] is a
+    value.
+
+  - The type [sequence t] is valid if and only if the type [t] is a
+    bounded type, i.e. [t] is either an array or a value type.
+
+ *)
+
+(*
+Inductive kind  := Unbounded | Bounded : bound -> kind
+with      bound := Array     | Value   : value -> bound
+with      value := Scalar    | Vector.
+
+(** Some short cuts to kinds. *)
+Definition valueK  (v : value) := Bounded (Value v).
+Definition scalarK := valueK Scalar.
+Definition vectorK := valueK Vector.
+Definition arrayK  := Bounded Array.
+ *)
+
+(**
+
+The inductive definition of types in verse.
+
+*)
+
+Inductive type       : Type :=
+| word               : nat -> type
+| vector             : nat -> type -> type
+| array              : nat -> endian -> type -> type
+| sequence           : type -> type
+with endian : Type := bigE | littleE | hostE.
+
+Inductive isValue : type ->  Prop :=
+| wordIsValue        {n : nat} : isValue (word n)
+| vectorIsValue      {n : nat}{t : type} :  isValue (vector n t)
+.
+
+Inductive isBounded : type -> Prop :=
+| wordIsBounded      {n : nat} : isBounded (word n)
+| vectorIsBounded    {n : nat}{t : type} : isBounded (vector n t)
+| arrayIsBounded     {n : nat}{e : endian}{t : type} : isBounded (array n e t)
+.
+
+(**
+
+* Size calculations.
+
+The number of bytes required to represent an element of
+a given type
+
+*)
+(*
+Require Import NPeano.
+Require Import Nat.
+
+Fixpoint bytes {b : bound}(t : type (Bounded b)) : nat :=
+  match t with
+    | word   n       => 2^n
+    | vector m w     => 2^m * bytes w
+    | array  n _ v   => n   * bytes v
+  end.
+
+Definition bits {b : bound}(t : type (Bounded b)) : nat
+  := 8 * bytes t.
+*)
+
